

This script verifies the (in)stability of the dynamical system formed by the Polyak stepsize with Mathematica.

```
In[ ]:= Clear["`*"];
```

Define functions and related assumptions.

```
In[ ]:= f[x_, y_] :=  $\frac{\kappa}{2} x^2 + \frac{1}{2} y^2$ ;
g[x_, y_] :=  $\begin{pmatrix} \kappa x \\ y \end{pmatrix}$ ;
alphapoly[x_, y_] :=  $\frac{f[x, y]}{\text{Norm}[g[x, y]]^2}$ ;
asp =  $x \in \mathbb{R} \wedge y > 0 \wedge 0 \leq \gamma \leq 2 \wedge \kappa > \frac{4 - \gamma}{\gamma} \wedge \kappa \geq 2$ ;
ResourceFunction["JacobianMatrix"];
```

Obtain the expression of the next state

```
In[ ]:=  $\begin{pmatrix} x \\ y \end{pmatrix} - \alpha g[x, y]$ 
Out[ ]:=  $\{ \{x - x \alpha \kappa\}, \{y - y \alpha\} \}$ 

In[ ]:= Simplify[ $\frac{\begin{pmatrix} x \\ y \end{pmatrix} - \alpha g[x, y]}{\text{Norm}[\begin{pmatrix} x \\ y \end{pmatrix} - \alpha g[x, y]]}$ , Assumptions -> asp &  $\alpha > 0$ ]
(* Next normalized point*)
Out[ ]:=  $\left\{ \left\{ \frac{x - x \alpha \kappa}{\sqrt{(y - y \alpha)^2 + (x - x \alpha \kappa)^2}} \right\}, \left\{ \frac{y - y \alpha}{\sqrt{(y - y \alpha)^2 + (x - x \alpha \kappa)^2}} \right\} \right\}$ 

In[ ]:= eplus =  $\gamma$  Simplify[alphapoly[x - x  $\alpha \kappa$ , y - y  $\alpha$ ], Assumptions -> asp &  $\alpha > 0$ ]
(*Next Polyak stepsize*)
Out[ ]:=  $\frac{\gamma (y^2 (-1 + \alpha)^2 + x^2 \kappa (-1 + \alpha \kappa)^2)}{2 (y^2 (-1 + \alpha)^2 + x^2 \kappa^2 (-1 + \alpha \kappa)^2)}$ 
```

Assemble the next state.

```
In[ ]:= s =  $\begin{pmatrix} \frac{x - x \alpha \kappa}{\sqrt{(y - y \alpha)^2 + (x - x \alpha \kappa)^2}} \\ \frac{y - y \alpha}{\sqrt{(y - y \alpha)^2 + (x - x \alpha \kappa)^2}} \\ \text{eplus} \end{pmatrix}$ ;
```

Solve for the initial conditions.

In[*]:= Solve $\left[\left\{x^2 = \frac{4 - \gamma (\kappa + 1)}{\gamma \kappa (\kappa + 1) - 4 \kappa^2} y^2, x^2 + y^2 = 1\right\}, \{x, y\}, \text{Reals}\right] // \text{Simplify}$

Out[*]=

$$\left\{ \left\{ x \rightarrow -\sqrt{\frac{4 - \gamma (1 + \kappa)}{(-4 + \gamma) (-1 + \kappa^2)}} \text{ if } \text{condition} \right\}, y \rightarrow -\sqrt{\frac{\kappa (\gamma - 4 \kappa + \gamma \kappa)}{(-4 + \gamma) (-1 + \kappa^2)}} \text{ if } \text{condition} \right\},$$

$$\left\{ x \rightarrow -\sqrt{\frac{4 - \gamma (1 + \kappa)}{(-4 + \gamma) (-1 + \kappa^2)}} \text{ if } \text{condition}, y \rightarrow \sqrt{\frac{\kappa (\gamma - 4 \kappa + \gamma \kappa)}{(-4 + \gamma) (-1 + \kappa^2)}} \text{ if } \text{condition} \right\},$$

$$\left\{ x \rightarrow \sqrt{\frac{4 - \gamma (1 + \kappa)}{(-4 + \gamma) (-1 + \kappa^2)}} \text{ if } \text{condition}, y \rightarrow -\sqrt{\frac{\kappa (\gamma - 4 \kappa + \gamma \kappa)}{(-4 + \gamma) (-1 + \kappa^2)}} \text{ if } \text{condition} \right\},$$

$$\left\{ x \rightarrow \sqrt{\frac{4 - \gamma (1 + \kappa)}{(-4 + \gamma) (-1 + \kappa^2)}} \text{ if } \text{condition}, y \rightarrow \sqrt{\frac{\kappa (\gamma - 4 \kappa + \gamma \kappa)}{(-4 + \gamma) (-1 + \kappa^2)}} \text{ if } \text{condition} \right\}$$

Evaluate the Jacobian matrix.

In[*]:= **JacobianMatrix** $\left[\left\{\frac{x - x \alpha \kappa}{\sqrt{(y - y \alpha)^2 + (x - x \alpha \kappa)^2}}, \frac{y - y \alpha}{\sqrt{(y - y \alpha)^2 + (x - x \alpha \kappa)^2}}, \text{eplus}\right\}, \{x, y, \alpha\}\right] // \text{FullSimplify} // \text{MatrixForm}$

Out[*]//MatrixForm=

$$\begin{pmatrix} -\frac{y^2 (-1+\alpha)^2 (-1+\alpha \kappa)}{((y-y \alpha)^2 + (x-x \alpha \kappa)^2)^{3/2}} & \frac{x y (-1+\alpha)^2 (-1+\alpha \kappa)}{((y-y \alpha)^2 + (x-x \alpha \kappa)^2)^{3/2}} & \frac{x y^2 (-1+\alpha) (-1+\kappa)}{((y-y \alpha)^2 + (x-x \alpha \kappa)^2)^{3/2}} \\ \frac{x y (-1+\alpha) (-1+\alpha \kappa)^2}{((y-y \alpha)^2 + (x-x \alpha \kappa)^2)^{3/2}} & -\frac{x^2 (-1+\alpha) (-1+\alpha \kappa)^2}{((y-y \alpha)^2 + (x-x \alpha \kappa)^2)^{3/2}} & -\frac{x^2 y (-1+\kappa) (-1+\alpha \kappa)}{((y-y \alpha)^2 + (x-x \alpha \kappa)^2)^{3/2}} \\ -\frac{x y^2 (-1+\alpha)^2 \gamma (-1+\kappa) \kappa (-1+\alpha \kappa)^2}{(y^2 (-1+\alpha)^2 + x^2 \kappa^2 (-1+\alpha \kappa)^2)^2} & \frac{x^2 y (-1+\alpha)^2 \gamma (-1+\kappa) \kappa (-1+\alpha \kappa)^2}{(y^2 (-1+\alpha)^2 + x^2 \kappa^2 (-1+\alpha \kappa)^2)^2} & \frac{x^2 y^2 (-1+\alpha) \gamma (-1+\kappa)^2 \kappa (-1+\alpha \kappa)}{(y^2 (-1+\alpha)^2 + x^2 \kappa^2 (-1+\alpha \kappa)^2)^2} \end{pmatrix}$$

Verify that the Polyak stepsize is unchanged after one iteration.

In[*]:= $\eta = \text{FullSimplify}[\gamma \text{alphapoly}[x, y] /. x \rightarrow -\sqrt{-\frac{y^2 (-4 + \gamma + \gamma \kappa)}{\kappa (\gamma - 4 \kappa + \gamma \kappa)}}, \text{Assumptions} \rightarrow \text{asp}]$

$\text{FullSimplify}[\text{eplus} /. \{x \rightarrow -\sqrt{-\frac{y^2 (-4 + \gamma + \gamma \kappa)}{\kappa (\gamma - 4 \kappa + \gamma \kappa)}}, \alpha \rightarrow \eta\}, \text{Assumptions} \rightarrow \text{asp}]$

Out[*]=

$$\frac{2}{1 + \kappa}$$

Out[*]=

eplus

Validate the spectrum of product Jacobians

$$\text{In[*]} := \mathbf{J} = \begin{pmatrix} -\frac{y^2 (-1+\alpha)^2 (-1+\alpha \kappa)}{((y-y \alpha)^2 + (x-x \alpha \kappa)^2)^{3/2}} & \frac{x y (-1+\alpha)^2 (-1+\alpha \kappa)}{((y-y \alpha)^2 + (x-x \alpha \kappa)^2)^{3/2}} & \frac{x y^2 (-1+\alpha) (-1+\kappa)}{((y-y \alpha)^2 + (x-x \alpha \kappa)^2)^{3/2}} \\ \frac{x y (-1+\alpha) (-1+\alpha \kappa)^2}{((y-y \alpha)^2 + (x-x \alpha \kappa)^2)^{3/2}} & -\frac{x^2 (-1+\alpha) (-1+\alpha \kappa)^2}{((y-y \alpha)^2 + (x-x \alpha \kappa)^2)^{3/2}} & -\frac{x^2 y (-1+\kappa) (-1+\alpha \kappa)}{((y-y \alpha)^2 + (x-x \alpha \kappa)^2)^{3/2}} \\ -\frac{x y^2 (-1+\alpha)^2 \gamma (-1+\kappa) \kappa (-1+\alpha \kappa)^2}{(y^2 (-1+\alpha)^2 + x^2 \kappa^2 (-1+\alpha \kappa)^2)^2} & \frac{x^2 y (-1+\alpha)^2 \gamma (-1+\kappa) \kappa (-1+\alpha \kappa)^2}{(y^2 (-1+\alpha)^2 + x^2 \kappa^2 (-1+\alpha \kappa)^2)^2} & \frac{x^2 y^2 (-1+\alpha) \gamma (-1+\kappa)^2 \kappa (-1+\alpha \kappa)}{(y^2 (-1+\alpha)^2 + x^2 \kappa^2 (-1+\alpha \kappa)^2)^2} \end{pmatrix};$$

```

In[*]:= J1 = FullSimplify[J /. {α → η, x → √(4 - γ (1 + κ) / (-4 + γ) (-1 + κ²)), y → √(κ (γ - 4 κ + γ κ) / (-4 + γ) (-1 + κ²))},
    Assumptions → asp];

J2 = FullSimplify[J /. {α → η, x → -√(4 - γ (1 + κ) / (-4 + γ) (-1 + κ²)), y → √(κ (γ - 4 κ + γ κ) / (-4 + γ) (-1 + κ²))},
    Assumptions → asp];

```

Case of $\gamma = 2$

```

In[*]:= M2 = FullSimplify[J2.J1 /. γ → 2, Assumptions → asp];

In[*]:= FullSimplify[Eigenvalues[M2], Assumptions → κ > 1]

Out[*]:= {0, 0, 1}

```

Case of $\gamma = 1$

```

In[*]:= M1 = FullSimplify[J2.J1 /. γ → 1, Assumptions → asp];
e1 = FullSimplify[Eigenvalues[M1], Assumptions → κ > 100];

```

```
In[*]:= e1
```

```
In[*]:= e1
```

```

Out[*]:= {
  2 Root[
    (
      (18 κ / √(-1 + κ²) - 126 κ² / √(-1 + κ²) + 162 κ³ / √(-1 + κ²) + 306 κ⁴ / √(-1 + κ²) - 306 κ⁵ / √(-1 + κ²) - 162 κ⁶ / √(-1 + κ²) + 126 κ⁷ / √(-1 + κ²) - 18 κ⁸ / √(-1 + κ²))
      #1² + #1³ &, 1
    ) / (9 (-1 + κ)⁴ κ (1 + κ) √(-1 + κ²)),
  2 Root[
    (
      (18 κ / √(-1 + κ²) - 126 κ² / √(-1 + κ²) + 162 κ³ / √(-1 + κ²) + 306 κ⁴ / √(-1 + κ²) - 306 κ⁵ / √(-1 + κ²) - 162 κ⁶ / √(-1 + κ²) + 126 κ⁷ / √(-1 + κ²) - 18 κ⁸ / √(-1 + κ²))
      #1² + #1³ &, 2
    ) / (9 (-1 + κ)⁴ κ (1 + κ) √(-1 + κ²)),
  2 Root[
    (
      (18 κ / √(-1 + κ²) - 126 κ² / √(-1 + κ²) + 162 κ³ / √(-1 + κ²) + 306 κ⁴ / √(-1 + κ²) - 306 κ⁵ / √(-1 + κ²) - 162 κ⁶ / √(-1 + κ²) + 126 κ⁷ / √(-1 + κ²) - 18 κ⁸ / √(-1 + κ²))
      #1² + #1³ &, 3
    ) / (9 (-1 + κ)⁴ κ (1 + κ) √(-1 + κ²))
}

```

The first two roots of the Polynomial are 0. Hence it suffices to consider the last one, with closed form given as follows.

```

In[*]:= v1 = -2 * (18 κ / √(-1 + κ²) - 126 κ² / √(-1 + κ²) + 162 κ³ / √(-1 + κ²) + 306 κ⁴ / √(-1 + κ²) - 306 κ⁵ / √(-1 + κ²) - 162 κ⁶ / √(-1 + κ²) + 126 κ⁷ / √(-1 + κ²) - 18 κ⁸ / √(-1 + κ²)) / (9 (-1 + κ)⁴ κ (1 + κ) √(-1 + κ²));

```

In[*]:= FullSimplify[v]

Out[*]=

$$\frac{4 (1 + (-4 + \kappa) \kappa)^2}{(-1 + \kappa)^4}$$

Solve for the final range of κ

Reduce $\left[\frac{4 (1 + (-4 + \kappa) \kappa)^2}{(-1 + \kappa)^4} > 1, \kappa\right]$

Out[*]=

$$\kappa < 3 - 2\sqrt{2} \mid \mid \frac{1}{3} < \kappa < 1 \mid \mid 1 < \kappa < 3 \mid \mid \kappa > 3 + 2\sqrt{2}$$